Substantial code cleanup that should have no computational effect. Linh, maybe you and I can chat a little about what changes I made and why.

inv_ack_hier.v
@@ -3,107 +3,110 @@ Require Import Setoid.
 
 
 (* USEFUL LEMMAS ABOUT NAT *)
+(** Can't these all be dealt with via Omega?
+ ** Why are we listing them again, and using them at all? 
+ **)
 Lemma le_add_le_sub_r : forall n m p : nat, n + p <= m -> n <= m - p.
-apply Nat.le_add_le_sub_r. Qed.
+Proof. apply Nat.le_add_le_sub_r. Qed.
 
 Lemma le_add_le_sub_l : forall n m p : nat, n + p <= m -> p <= m - n.
-apply Nat.le_add_le_sub_l. Qed.
+Proof. apply Nat.le_add_le_sub_l. Qed.
 
 Lemma lt_add_lt_sub_r : forall n m p : nat, n + p < m <-> n < m - p.
-apply Nat.lt_add_lt_sub_r. Qed.
+Proof. apply Nat.lt_add_lt_sub_r. Qed.
 
 Lemma lt_add_lt_sub_l : forall n m p : nat, n + p < m <-> p < m - n.
-apply Nat.lt_add_lt_sub_l. Qed.
+Proof. apply Nat.lt_add_lt_sub_l. Qed.
 
 Lemma lt_le_S : forall n m : nat, n < m <-> S n <= m.
-intros. omega. Qed.
+Proof. intros. omega. Qed.
 
 Lemma minus_n_0 : forall n, n - 0 = n.
-intros. rewrite minus_n_O. trivial. Qed.
+Proof. intros. rewrite minus_n_O. trivial. Qed.
 
 Lemma sub_add_distr: forall n m p : nat, n - (m + p) = n - m - p.
-intros. apply Nat.sub_add_distr. Qed.
+Proof. intros. apply Nat.sub_add_distr. Qed.
 
 Lemma sub_sub_comm: forall n m p: nat, n - m - p = n - p - m.
-intros. rewrite <- sub_add_distr. rewrite <- sub_add_distr.
-rewrite plus_comm. trivial. Qed.
+Proof.
+  intros. rewrite <- sub_add_distr, <- sub_add_distr, plus_comm.
+  trivial.
+Qed.
 
 Lemma add_sub_eq_l: forall n m p : nat, m + p = n -> n - m = p.
-apply Nat.add_sub_eq_l. Qed.
+Proof.  apply Nat.add_sub_eq_l. Qed.
 
 Lemma add_sub_eq_r: forall n m p : nat, m + p = n -> n - p = m.
-apply Nat.add_sub_eq_r. Qed.
+Proof. apply Nat.add_sub_eq_r. Qed.
 
 Lemma le_plus_minus: forall n m : nat, n <= m -> m = n + (m - n).
-apply le_plus_minus. Qed.
+  apply le_plus_minus. Qed.
 
 Lemma minus_S : forall n m : nat, n - m = S n - S m.
-intros. omega. Qed.
+Proof. intros. omega. Qed.
 
 Lemma le_S_n_m : forall n m : nat, n <= m <-> S n <= S m.
-split. apply Peano.le_n_S. apply Peano.le_S_n. Qed.
+Proof. split. apply Peano.le_n_S. apply Peano.le_S_n. Qed.
 
 Lemma lt_S_n_m : forall n m : nat, n < m <-> S n < S m.
-intros. omega. Qed.
+Proof. intros. omega. Qed.
 
 Lemma sub_compl: forall n m : nat, m <= n -> n - (n - m) = m.
-intros. apply add_sub_eq_r. symmetry. apply le_plus_minus. trivial. Qed.
+Proof.
+  intros. apply add_sub_eq_r. symmetry.
+  apply le_plus_minus. trivial.
+Qed.
 
 Lemma sub_lt: forall n m : nat, m <= n -> 0 < m -> n - m < n.
-apply Nat.sub_lt. Qed.
+Proof. apply Nat.sub_lt. Qed.
 
 Lemma le_sub_l: forall n m : nat, n - m <= n.
-apply Nat.le_sub_l. Qed.
+Proof. apply Nat.le_sub_l. Qed.
 
 Lemma le_succ_l: forall n m : nat, S n <= m <-> n < m.
-apply Nat.le_succ_l. Qed.
+Proof. apply Nat.le_succ_l. Qed.
 
 Lemma lt_succ_r: forall n m : nat, n < S m <-> n <= m.
-apply Nat.lt_succ_r. Qed.
+Proof. apply Nat.lt_succ_r. Qed.
 
 Lemma lt_lt_0: forall n m : nat, n < m -> 0 < m.
-apply Nat.lt_lt_0. Qed.
+Proof. apply Nat.lt_lt_0. Qed.
 
 Lemma le_cases: forall n m : nat, n <= m -> (n <= m-1 \/ (n = m /\ m <> 0)).
-intros. destruct H.
-- destruct n. simpl. left. omega. right. omega.
-- simpl. rewrite minus_n_0. left. trivial.
-Qed.
+Proof. intros. destruct H; omega. Qed.
 
 Lemma nat_compare: forall n m : nat, S n <= m \/ n = m \/ S m <= n.
-intros. assert (H := le_lt_dec m n). destruct H as [H1 | H2].
-- right. inversion H1. omega. right. omega.
-- left. omega.
-Qed.
+Proof. intros. omega. Qed.
 
 Lemma not_lt: forall n m : nat, n <= m <-> ~ m < n.
-split. omega. omega. Qed.
+Proof. split. omega. omega. Qed.
 
 Lemma not_le: forall n m : nat, ~ n <= m <-> m < n.
-split. omega. omega. Qed.
+Proof. split. omega. omega. Qed.
 
 Lemma le_antisymm: forall n m : nat, n <= m -> m <= n -> n = m.
-apply le_antisym. Qed.
+Proof. apply le_antisym. Qed.
 
 
 
 (* LEMMAS ABOUT DECREASING FUNCTIONS *)
 
-Fixpoint repeat (f: nat -> nat) (rep n : nat) : nat
-:= match rep with
-   | 0      => n
-   | S rep' => f (repeat f rep' n)
-end.
+Fixpoint repeat (f: nat -> nat) (rep n : nat) : nat :=
+  match rep with
+  | 0 => n
+  | S rep' => f (repeat f rep' n)
+  end.
 
 Theorem repeat_S_comm : forall f k n, repeat f (S k) n = repeat f k (f n).
 Proof.
-induction k. { trivial. }
-intro. simpl. simpl in IHk. rewrite IHk. trivial.
+  induction k; trivial.
+  intro. simpl in *; rewrite IHk; trivial.
 Qed.
 
-Definition shrinking (f : nat -> nat) := forall m, f m <= m - 1.
+Definition shrinking (f : nat -> nat) :=
+  forall m, f m <= m - 1.
 
-(* A couple examples of the kind of proof cleanup I think we could do *)
+(** A couple examples of the kind of proof cleanup I think we could do **)
 Theorem repeat_shrinking : forall f k l n,
     (shrinking f) -> (k < l) -> (repeat f l n <= repeat f k n - 1).
 Proof.
@@ -116,70 +119,50 @@ Proof.
   - induction l; [inversion 1|].
     intro. inversion H0; [subst; simpl; trivial|].
     apply (Nat.le_trans _ (repeat f l n) _); [simpl | apply IHl; omega].
-    apply (Nat.le_trans _ (repeat f l n - 1) _); [apply H|omega].
+    apply (Nat.le_trans _ (repeat f l n - 1) _); [apply H | omega].
 Qed.
 
 Theorem shrink_threshold : forall f n t,
-    (shrinking f) ->
-    (n > t) ->
-    (exists k, (repeat f (S k) n <= t) /\ (t < repeat f k n)).
-Proof.
-  Theorem shrink_threshold : forall f n t,
-(shrinking f) ->
-(n > t) ->
-(exists k, (repeat f (S k) n <= t) /\ (t < repeat f k n)).
+    shrinking f ->
+    n > t ->
+    exists k, repeat f (S k) n <= t /\ t < repeat f k n.
 Proof.
   intros f n t Hf Hn.
-  assert (n = (n - t) + t) by omega.
   remember (n - t) as l.
-  assert (t = n - l) by omega.
-  rewrite H0.
-  clear Heql. clear H.
-  assert (l <> 0) by omega.
-  clear H0.
-  destruct l. omega.
-  clear H.
-  induction l.
-  - exists 0. split.
-    replace (n - 1) with (repeat f 0 n - 1). apply Hf. trivial.
-    simpl. apply sub_lt. rewrite le_succ_l. apply (lt_lt_0 t n). trivial. omega.
-  - assert (n - S(S l) = n - S l - 1) by omega.
+  replace t with (n - l) by omega; destruct l; [omega|].
+  clear Heql. induction l.
+  - exists 0.
+    replace (n - 1) with (repeat f 0 n - 1) by trivial.
+    split; [apply Hf | simpl; omega].
+  - assert (n - S (S l) = n - S l - 1) by omega.
     rewrite H. remember (n - S l) as s.
     destruct IHl as [h Hs]. destruct Hs as [Hs1 Hs2].
     apply le_cases in Hs1. destruct Hs1 as [Hs1 | Hs1].
-    + exists h. split. trivial. rewrite <- le_succ_l in Hs2. rewrite <- le_succ_l.
-      apply (Nat.le_trans _ (S s) _). apply Peano.le_n_S. apply le_sub_l. trivial.
+    + exists h. split; trivial. omega.
     + destruct Hs1 as [Hs0 Hs1]. exists (S h). simpl. split.
       * rewrite <- Hs0. apply Hf.
-      * simpl in Hs0. rewrite Hs0. destruct s.
-        exfalso. apply Hs1. trivial.
-        simpl. rewrite minus_n_0. apply Nat.lt_succ_diag_r.
+      * simpl in Hs0; rewrite Hs0; omega. 
 Qed.
 
 Lemma repeat_shrink : forall f, shrinking f -> (forall n k, repeat f k n <= n - k).
 Proof.
-intros f Hf n. induction k.
-- simpl. omega.
-- simpl. apply (Nat.le_trans _ (repeat f k n - 1) _). apply Hf. omega.
+  intros f Hf n. induction k; simpl; [omega|]. 
+  apply (Nat.le_trans _ (repeat f k n - 1) _); [apply Hf | omega].
 Qed.
-
 
 Lemma shrink_f_0 : forall f, (shrinking f) -> (forall k, repeat f k 0 = 0).
 Proof.
-induction k. trivial.
-simpl. rewrite IHk.
-assert (f 0 <= 0). { apply H. } inversion H0. rewrite H2. rewrite H2. trivial.
+  induction k; trivial.
+  simpl. rewrite IHk.
+  assert (f 0 <= 0) by apply H; inversion H0. auto.
 Qed.
-
 
 Lemma shrink_f_1 : forall f, (shrinking f) -> (forall k, repeat f (S k) 1 = 0).
 Proof.
-induction k. simpl.
-specialize (H 1). inversion H. rewrite H1. trivial.
-replace (repeat f (S (S k)) 1) with (f (repeat f (S k) 1)).
-rewrite IHk.
-specialize (H 0). inversion H. rewrite H1. trivial.
-trivial.
+  induction k.
+  - specialize (H 1); inversion H; rewrite H1; trivial.
+  - replace (repeat f (S (S k)) 1) with (f (repeat f (S k) 1)) by trivial.
+    rewrite IHk; specialize (H 0); inversion H; rewrite H1; trivial.
 Qed.
 
 
@@ -187,21 +170,22 @@ Qed.
 ========= DEFINITIONS ============================ *)
 
 Fixpoint next_level_worker (f : nat -> nat) (n n1 cd : nat) : nat
-:=
-match n with
-| 0 => 0
-| 1 => 0
-| S n' => match n1 with
-          | 0 => 1
-          | 1 => 1
-          | _ =>
-          match cd with
-          | 0 => match (f n1) with | n2 => S(next_level_worker f n' n2 (n1 - n2 - 1)) end
-          | S cd' => next_level_worker f n' n1 cd'
-          end
-          end
-end.
+  :=
+    match n with
+    | 0 => 0
+    | 1 => 0
+    | S n' => match n1 with
+              | 0 => 1
+              | 1 => 1
+              | _ =>
+                match cd with
+                | 0 => match (f n1) with | n2 => S(next_level_worker f n' n2 (n1 - n2 - 1)) end
+                | S cd' => next_level_worker f n' n1 cd'
+                end
+              end
+    end.
 
+(** Anshuman's version: **)
 Fixpoint next_level_worker' (f : nat -> nat) (n n1 cd : nat) : nat :=
   match n, n1 with
   | 0, _ => 0
@@ -210,32 +194,30 @@ Fixpoint next_level_worker' (f : nat -> nat) (n n1 cd : nat) : nat :=
   | _, 1 => 1
   | S n', _ =>
     match cd with
-    | 0 => match (f n1) with | n2 => S(next_level_worker f n' n2 (n1 - n2 - 1)) end
-    | S cd' => next_level_worker f n' n1 cd'
+    | 0 => S (next_level_worker' f n' (f n1) (n1 - f n1 - 1))
+    | S cd' => next_level_worker' f n' n1 cd'
     end
   end.
 
-Definition next_level f n
-:= match (f n) with | n1 => next_level_worker f n n1 (n - n1 - 1)
-end.
+Definition next_level f n := next_level_worker f n (f n) (n - f n - 1).
 
-(* example of potential cleanup *)
+
+(** example of potential cleanup **)
 
 Definition next_level_fast f n
-:= match n with
-   | 0 => 0
-   | 1 => 0
-   | _ => match (f n) with
-          | n1 => S(next_level f n1) end
-end.
+  := match n with
+     | 0 => 0
+     | 1 => 0
+     | _ => match (f n) with
+            | n1 => S(next_level f n1) end
+     end.
 
 Definition next_level_fast' f n :=
   match n with
-  | 0 => 0
-  | 1 => 0
+  | 0 | 1 => 0
   | _ => S (next_level f (f n))
   end.
-  
+
 Definition sub2 (n : nat) : nat := n - 2.
 
 Compute sub2 2.
@@ -253,36 +235,39 @@ Compute next_level sub2 4.
 (* LEMMAS ABOUT NEXT_LEVEL_WORKER *)
 
 Lemma next_level_interstate_1 : forall f n n1 cd k,
-(2 <= n1) -> (k <= cd) -> (k <= n)
--> next_level_worker f n n1 cd = next_level_worker f (n - k) n1 (cd - k).
+    2 <= n1 ->
+    k <= cd ->
+    k <= n ->
+    next_level_worker f n n1 cd = next_level_worker f (n - k) n1 (cd - k).
 Proof.
-intros f n n1 cd k Hn1. generalize dependent cd.
-generalize dependent k. induction n. { trivial. }
-intros k cd Hk Hkn1. destruct k. { repeat rewrite minus_n_0. trivial. }
-destruct cd. { inversion Hk. }
-apply le_S_n_m in Hk. repeat rewrite Nat.sub_succ. rewrite <- le_S_n_m in Hkn1.
-rewrite <- IHn.
-- destruct n. trivial.
-  destruct n1. inversion Hn1. destruct n1. inversion Hn1. inversion H0.
-  trivial.
-- trivial.
-- trivial.
+  intros f n n1 cd k Hn1. generalize dependent cd.
+  generalize dependent k. induction n; trivial.
+  intros k cd Hk Hkn1.
+  destruct k; [repeat rewrite minus_n_0; trivial|]. 
+  destruct cd; [inversion Hk|].
+  apply le_S_n_m in Hk. rewrite <- le_S_n_m in Hkn1.
+  repeat rewrite Nat.sub_succ. rewrite <- (IHn _ _ Hk Hkn1).
+  destruct n; trivial.
+  destruct n1; [inversion Hn1|].
+  destruct n1; [inversion Hn1; inversion H0|]; trivial. 
 Qed.
 
-
 Lemma next_level_interstate_2 : forall f n,
-shrinking f -> 2 <= n -> next_level f n = 1 + next_level f (f n).
+    shrinking f ->
+    2 <= n ->
+    next_level f n = 1 + next_level f (f n).
 Proof.
-intros. unfold next_level. destruct n. inversion H0.
-destruct n. inversion H0. inversion H2.
-remember (f (S (S n))) as n1.
-destruct n1. { trivial. } destruct n1. { trivial. }
-remember (S (S n) - S (S n1) - 1) as cd.
-rewrite (next_level_interstate_1 _ _ _ _ cd). rewrite Nat.sub_diag.
-assert (S(S n) - cd = (S (S (S n1)))).
-{ rewrite Heqcd. rewrite <- sub_add_distr. rewrite plus_comm. rewrite sub_compl.
-  trivial. rewrite <- le_S_n_m. rewrite Heqn1. apply H. }
-rewrite H1. trivial. omega. trivial. omega.
+  intros. unfold next_level. destruct n; [inversion H0|].
+  destruct n; [inversion H0; inversion H2|].
+  remember (f (S (S n))) as n1.
+  destruct n1; trivial. destruct n1; trivial.
+  remember (S (S n) - S (S n1) - 1) as cd.
+  rewrite (next_level_interstate_1 _ _ _ _ cd); [|omega | trivial | omega].
+  rewrite Nat.sub_diag.
+  assert (S (S n) - cd = (S (S (S n1)))). 
+  { rewrite Heqcd. rewrite <- sub_add_distr, plus_comm, sub_compl; trivial.
+    rewrite <- le_S_n_m. rewrite Heqn1. apply H. }
+  rewrite H1. trivial.
 Qed.
 
 
@@ -291,34 +276,20 @@ Qed.
 (* Another example *)
 
 Theorem next_level_repeat_1 : forall f n k,
-shrinking f -> (repeat f k n <= 1 <-> next_level f n <= k).
-Proof.
-intros. generalize dependent n. induction k.
-{ intro n. simpl. destruct n. { unfold next_level. simpl. omega. }
-  destruct n. { unfold next_level. simpl. omega. }
-  rewrite next_level_interstate_2. omega. trivial. omega. }
-intro n.
-destruct n. { unfold next_level. rewrite shrink_f_0. simpl. omega. trivial. }
-destruct n. { unfold next_level. rewrite shrink_f_1. simpl. omega. trivial. }
-rewrite repeat_S_comm. rewrite next_level_interstate_2. rewrite <- le_S_n_m.
-apply IHk. trivial. omega.
-Qed.
-
-
-Theorem next_level_repeat_1' : forall f n k,
     shrinking f ->
     repeat f k n <= 1 <-> next_level f n <= k.
 Proof.
-  intros. generalize dependent n. induction k.
-  - intro n. simpl. destruct n; [unfold next_level; simpl; omega|].
-    destruct n; [unfold next_level; simpl; omega|].
-    rewrite next_level_interstate_2; [omega | trivial | omega].
-  - intro n; destruct n.
+  intros. generalize dependent n. induction k; intro n.
+  - simpl. destruct n.
+    + unfold next_level. simpl; omega.
+    + destruct n; [now unfold next_level|]. 
+      rewrite next_level_interstate_2; [omega | trivial | omega].
+  - destruct n.
     + unfold next_level. rewrite shrink_f_0; [simpl; omega | trivial].
-    + destruct n; [unfold next_level; rewrite shrink_f_1; trivial; simpl; omega|]. 
-      rewrite repeat_S_comm.
-      rewrite next_level_interstate_2; [|trivial | omega].
-      rewrite <- le_S_n_m; trivial.
+    + destruct n.
+      * unfold next_level. rewrite shrink_f_1; [simpl; omega | trivial].
+      * rewrite repeat_S_comm, next_level_interstate_2, <- le_S_n_m;
+          [trivial | trivial | omega].
 Qed.
 
 Theorem next_level_repeat_2 : forall (f : nat -> nat) (n k : nat),
@@ -326,26 +297,27 @@ Theorem next_level_repeat_2 : forall (f : nat -> nat) (n k : nat),
     next_level f n = k <->
     repeat f k n <= 1 /\ forall p, repeat f p n <= 1 -> k <= p. 
 Proof.
-intros f n k Hf. split.
-- intro Hk. split.
-  + rewrite next_level_repeat_1. omega. trivial.
-  + intros p Hp. rewrite <- Hk. rewrite <- next_level_repeat_1; trivial.
-- intro Hk. destruct Hk as [Hk1 Hk2].
-  apply le_antisym. rewrite <- next_level_repeat_1; trivial.
-  apply (Hk2 (next_level f n)). rewrite next_level_repeat_1; trivial. 
+  intros f n k Hf. split.
+  - intro Hk. split.
+    + rewrite next_level_repeat_1; [omega | trivial].
+    + intros p Hp. rewrite <- Hk, <- next_level_repeat_1; trivial.
+  - intro Hk. destruct Hk as [Hk1 Hk2].
+    apply le_antisym.
+    + rewrite <- next_level_repeat_1; trivial.
+    + apply (Hk2 (next_level f n)); rewrite next_level_repeat_1; trivial. 
 Qed.
 
 
 (* PROPER SHRINKING PRESERVE THEOREM *)
 
 Theorem next_level_shrink : forall f,
-shrinking f -> shrinking (next_level f).
+    shrinking f -> shrinking (next_level f).
 Proof.
-intros f Hf. unfold shrinking.
-intros. rewrite <- next_level_repeat_1.
-assert (forall n k, repeat f k n <= n - k).
-{ apply repeat_shrink. trivial. }
-specialize (H m (m - 1)). omega. trivial.
+  intros f Hf. unfold shrinking.
+  intros. rewrite <- next_level_repeat_1; trivial.
+  assert (forall n k, repeat f k n <= n - k) by
+      (apply repeat_shrink; trivial).
+  specialize (H m (m - 1)); omega.
 Qed.
 
 
@@ -355,101 +327,106 @@ Definition increasing (f : nat -> nat) : Prop := forall n m, n <= m -> f n <= f 
 
 Definition increasing_strict (f : nat -> nat) : Prop := forall n m, n < m -> f n < f m.
 
-
 Lemma incr_S : forall f, increasing f <-> (forall n, f n <= f (S n)).
 Proof.
-intro. split. { intros. apply H. omega. }
-{ unfold increasing. intros. generalize dependent n. induction m.
-- intros. inversion H0. omega.
-- intros. inversion H0. omega. apply IHm in H2. apply (Nat.le_trans _ (f m) _).
-  trivial. apply H. }
+  intro. split.
+  - intros. apply H. omega.
+  - unfold increasing. intros. generalize dependent n.
+    induction m; intros; inversion H0; [omega | omega|].
+    intros. inversion H0. omega. apply IHm in H2. apply (Nat.le_trans _ (f m) _); [trivial | apply H]. 
 Qed.
-
 
 Lemma incr_strict_S : forall f, increasing_strict f <-> (forall n, f n < f (S n)).
 Proof.
-intro. split. { intros. apply H. omega. }
-{ unfold increasing_strict. intros. generalize dependent n. induction m.
-- intros. inversion H0.
-- intros. inversion H0. apply H. apply IHm in H2. apply (Nat.lt_trans _ (f m) _).
-  trivial. apply H. }
+  intro. split.
+  - intros. apply H. omega.
+  - unfold increasing_strict. intros. generalize dependent n. induction m.
+    + intros. inversion H0.
+    + intros. inversion H0; [apply H|].
+      apply IHm in H2. apply (Nat.lt_trans _ (f m) _); [trivial | apply H].
 Qed.
-
 
 Lemma repeat_incr : forall f, increasing f -> (forall k, increasing (repeat f k)).
 Proof.
-intro f. unfold increasing. intro Hf.
-induction k. simpl. intros. trivial.
-intros. simpl. apply Hf. apply IHk. trivial.
+  intro f. unfold increasing. intro Hf.
+  induction k.
+  - simpl. intros. trivial.
+  - intros. simpl. apply Hf. apply IHk. trivial.
 Qed.
 
-
 Theorem next_level_incr : forall f,
-shrinking f -> increasing f -> increasing (next_level f).
+    shrinking f ->
+    increasing f ->
+    increasing (next_level f).
 Proof.
-intros f Hf0 Hf1 n m Hnm. apply next_level_repeat_1. trivial.
-assert (increasing (repeat f (next_level f m))).
-{ apply repeat_incr. trivial. }
-specialize (H n m). apply H in Hnm.
-apply (Nat.le_trans _ (repeat f (next_level f m) m) _).
-trivial. apply next_level_repeat_1. trivial. trivial.
+  intros f Hf0 Hf1 n m Hnm. apply next_level_repeat_1; trivial.
+  assert (increasing (repeat f (next_level f m))) by
+      (apply repeat_incr; trivial). 
+  apply (H n m) in Hnm.
+  apply (Nat.le_trans _ (repeat f (next_level f m) m) _); trivial.
+  apply next_level_repeat_1; trivial.
 Qed.
 
 
 (* THE ACKERMANN HIERARCHY *)
 
 Definition can_inv_rel (f F : nat -> nat) : Prop
-:= forall n N, f N <= n <-> N <= F n.
+  := forall n N, f N <= n <-> N <= F n.
 
 Fixpoint next_can_level F n : nat :=
-match n with
-| 0 => 1
-| S n' => F (next_can_level F n')
-end.
-
+  match n with
+  | 0 => 1
+  | S n' => F (next_can_level F n')
+  end.
 
 Definition growing (F : nat -> nat) : Prop := forall n, S n <= F n.
 
-
-Lemma can_inv_growing : forall f F, shrinking f -> can_inv_rel f F -> growing F.
+Lemma can_inv_growing : forall f F,
+    shrinking f ->
+    can_inv_rel f F ->
+    growing F.
 Proof.
-intros f F Hf HfF n. rewrite <- (HfF n _).
-apply (Nat.le_trans _ (S n - 1) _). apply Hf. omega.
+  intros f F Hf HfF n. rewrite <- (HfF n _).
+  apply (Nat.le_trans _ (S n - 1) _); [apply Hf | omega].
 Qed.
-
 
 Lemma can_inv_positive : forall f F,
-shrinking f -> can_inv_rel f F -> (forall n, 0 < F n).
+    shrinking f ->
+    can_inv_rel f F ->
+    forall n, 0 < F n.
 Proof.
-intros f F Hf HfF n. apply (Nat.le_trans _ (S n) _). omega.
-generalize dependent n. apply (can_inv_growing f F). trivial. trivial.
+  intros f F Hf HfF n. apply (Nat.le_trans _ (S n) _); [omega|].
+  generalize dependent n. apply (can_inv_growing f F); trivial. 
 Qed.
 
-
 Lemma can_inv_increasing : forall f F,
-shrinking f -> increasing f -> can_inv_rel f F -> increasing F.
+    shrinking f ->
+    increasing f ->
+    can_inv_rel f F ->
+    increasing F.
 Proof.
-intros f F Hf_sh Hf_in HfF. rewrite incr_S. intro.
-rewrite <- (HfF (S n) _). apply (Nat.le_trans _ n _).
-rewrite (HfF n _). trivial. omega.
+  intros f F Hf_sh Hf_in HfF. rewrite incr_S. intro.
+  rewrite <- (HfF (S n) _). apply (Nat.le_trans _ n _).
+  rewrite (HfF n _). trivial. omega.
 Qed.
 
 
 Theorem inv_next_level_can : forall f F,
-shrinking f -> increasing f -> can_inv_rel f F
--> can_inv_rel (next_level f) (next_can_level F).
+    shrinking f ->
+    increasing f ->
+    can_inv_rel f F ->
+    can_inv_rel (next_level f) (next_can_level F).
 Proof.
-intros f F Hf1 Hf2 HfF. unfold can_inv_rel.
-induction n.
-{ simpl. intro. rewrite <- next_level_repeat_1. simpl. omega. trivial. }
-intro. simpl.
-destruct N. { unfold next_level. simpl. omega. }
-destruct N.
-{ unfold next_level. simpl. split.
-  - intro. apply (can_inv_positive f F). trivial. trivial.
-  - intro. omega. }
-rewrite next_level_interstate_2. rewrite <- le_S_n_m.
-rewrite (IHn (f (S (S N)))). apply HfF. trivial. omega.
+  intros f F Hf1 Hf2 HfF. unfold can_inv_rel.
+  induction n.
+  - simpl. intro. rewrite <- next_level_repeat_1; [simpl; omega | trivial].
+  - intro. simpl. destruct N; [unfold next_level; simpl; omega|].
+    destruct N.
+    + unfold next_level. simpl. split.
+      * intro. apply (can_inv_positive f F); trivial. 
+      * omega. 
+    + rewrite next_level_interstate_2, <- le_S_n_m; [|trivial | omega].
+      rewrite (IHn (f (S (S N)))). apply HfF.
 Qed.
 
 
@@ -502,7 +479,7 @@ Proof. intro. rewrite minus_2_correct. omega. Qed.
 
 Theorem minus_b_shrink: forall b, 0 < b -> shrinking (minus_b b).
 Proof. unfold minus_b, shrinking. intros. omega. Qed.
- 
+
 (* HIGHER LEVELS *)
 
 (* I think you want minus_b here *)
@@ -521,32 +498,32 @@ Fixpoint inv_ack_hier_b b i n :=
 
 Fixpoint ack_hier i n :=
   match i with
-   | 0 => S (S n)
-   | S i' => next_can_level (ack_hier i') n
-end.
+  | 0 => S (S n)
+  | S i' => next_can_level (ack_hier i') n
+  end.
 
 Fixpoint ack_hier_b b i n :=
   match i with
-   | 0 => n + b
-   | S i' => next_can_level (ack_hier_b b i') n
+  | 0 => n + b
+  | S i' => next_can_level (ack_hier_b b i') n
   end.
 
 Fixpoint inv_ack_hier_fast i n :=
   match i with
-   | 0 => minus_2 n
-   | S i' => next_level_fast (inv_ack_hier i') n
-   end.
-(* Two things, 
+  | 0 => minus_2 n
+  | S i' => next_level_fast (inv_ack_hier i') n
+  end.
+(** Two things, 
    1. how about
       S i' => next_level_fast (inv_ack_hier_fast i') n
    2. how about minus_b instead? 
- *)
+ **)
 
-(* trying both of these below... *)
+(** trying both of these below... **)
 Fixpoint inv_ack_hier_faster_b b i n :=
   match i with
-   | 0 => minus_b b n
-   | S i' => next_level_fast (inv_ack_hier_faster_b b i') n
+  | 0 => minus_b b n
+  | S i' => next_level_fast (inv_ack_hier_faster_b b i') n
   end.
 
 Lemma issame: forall f n,
@@ -617,235 +594,256 @@ Corollary inv_ack_hier_each_shrink_b : forall b i, 0 < b -> shrinking (inv_ack_h
 Qed.
 
 Corollary inv_ack_hier_shrink : forall i n,
-(3 <= n) -> (inv_ack_hier (S i) n) <= inv_ack_hier i n.
+    (3 <= n) -> (inv_ack_hier (S i) n) <= inv_ack_hier i n.
 Proof.
-intros. assert (Hi := (inv_ack_hier_each_shrink i)). simpl.
-rewrite <- next_level_repeat_1. remember (inv_ack_hier i n) as m.
-destruct m.
-- simpl. destruct i. { simpl in Heqm. rewrite minus_2_correct in Heqm. omega. }
-  symmetry in Heqm. simpl in Heqm. rewrite next_level_repeat_2 in Heqm.
-  destruct Heqm as [Heqm _]. simpl in Heqm. trivial. apply inv_ack_hier_each_shrink.
-- rewrite repeat_S_comm. apply (Nat.le_trans _ (inv_ack_hier i n - m) _).
-  apply repeat_shrink. trivial. omega.
-- trivial.
+  intros. assert (Hi := (inv_ack_hier_each_shrink i)). simpl.
+  rewrite <- next_level_repeat_1 by trivial.
+  remember (inv_ack_hier i n) as m; destruct m.
+  - simpl. destruct i.
+    + simpl in Heqm. rewrite minus_2_correct in Heqm. omega.
+    + symmetry in Heqm. simpl in Heqm. rewrite next_level_repeat_2 in Heqm.
+      * destruct Heqm as [Heqm _]. simpl in Heqm. trivial.
+      * apply inv_ack_hier_each_shrink.
+  - rewrite repeat_S_comm. apply (Nat.le_trans _ (inv_ack_hier i n - m) _);
+                             [apply repeat_shrink; trivial | omega].
 Qed.
 
-
 Corollary inv_ack_hier_shrink_gen : forall i j n,
-(3 <= n) -> (i <= j) -> (inv_ack_hier j n) <= inv_ack_hier i n.
+    3 <= n ->
+    i <= j ->
+    inv_ack_hier j n <= inv_ack_hier i n.
 Proof.
-intros i j n Hn Hij. generalize dependent i.
-induction j. { intros. inversion Hij. trivial. }
-intros. inversion Hij.
-{ trivial. }
-apply (Nat.le_trans _ (inv_ack_hier j n) _).
-{ apply inv_ack_hier_shrink. trivial. }
-apply IHj. trivial.
+  intros i j n Hn Hij. generalize dependent i.
+  induction j.
+  - intros. inversion Hij. trivial.
+  - intros. inversion Hij; trivial.
+    apply (Nat.le_trans _ (inv_ack_hier j n) _);
+      [apply inv_ack_hier_shrink | apply IHj]; trivial.
 Qed.
 
 
 (* RELATION TO ACKERMANN FUNCTION *)
 
-
 Fixpoint next_ack_level f n : nat :=
-match n with
-| 0 => f 1
-| S n' => f (next_ack_level f n')
-end.
-
+  match n with
+  | 0 => f 1
+  | S n' => f (next_ack_level f n')
+  end.
 
 Fixpoint Ack m n : nat :=
-match m with
-| 0 => S n
-| S m' => next_ack_level (Ack m') n
-end.
-
+  match m with
+  | 0 => S n
+  | S m' => next_ack_level (Ack m') n
+  end.
 
 Lemma Ack_1 : forall n, Ack 1 n = n + 2.
 Proof.
-induction n. trivial. unfold Ack. simpl. unfold Ack in IHn. rewrite IHn. trivial.
+  induction n; trivial.
+  unfold Ack. simpl. unfold Ack in IHn. rewrite IHn; trivial.
 Qed.
-
 
 Lemma ack_hier_1 : forall m, ack_hier m 1 = 3.
 Proof. induction m; trivial. Qed.
 
 Theorem ack_hier_Ack : forall m n, ack_hier m (n + 2) = Ack (m + 1) n + 2.
 Proof.
-induction m.
-{ intro. rewrite Ack_1. simpl. omega. }
-induction n.
-{ simpl. rewrite <- (IHm 1). rewrite ack_hier_1. trivial. }
-simpl. simpl in IHn. rewrite IHn. rewrite IHm. trivial.
+  induction m.
+  - intro. rewrite Ack_1. simpl. omega.
+  - induction n; simpl.
+    + rewrite <- (IHm 1). rewrite ack_hier_1. trivial. 
+    + simpl in IHn. rewrite IHn. rewrite IHm. trivial.
 Qed.
 
-
 Theorem inv_ack_Ack : forall n x y,
-n <= Ack (S x) y <-> inv_ack_hier x (n + 2) <= y + 2.
+    n <= Ack (S x) y <-> inv_ack_hier x (n + 2) <= y + 2.
 Proof.
-intros. assert (inv_ack_like_rel (inv_ack_hier x) (ack_hier x)).
-{ apply inv_hier_ack_hier. }
-destruct H as [_ H]. destruct H as [_ H]. destruct H as [H _].
-rewrite (H (y+2) (n+2)). rewrite ack_hier_Ack.
-replace (x+1) with (S x). omega. omega.
+  intros. assert (inv_ack_like_rel (inv_ack_hier x) (ack_hier x)) by
+      apply inv_hier_ack_hier. 
+  destruct H as [_ [_ [H _]]]. 
+  rewrite (H (y+2) (n+2)). rewrite ack_hier_Ack.
+  replace (x+1) with (S x); omega. 
 Qed.
 
 
 (* INVERSE ACKERMANN DEFINITION *)
 
-Definition inv_ack_rel n a := forall x, n <= Ack x x <-> a <= x.
-
+Definition inv_ack_rel n a := forall x,
+    n <= Ack x x <-> a <= x.
 
 (* Find minimum u such that inv_ack_hier u n <= u + 3 *)
 Fixpoint inv_ack_worker n f cd1 cd0 :=
-match cd0 with
-| 0 => 0
-| 1 => 1
-| S cd0' => match cd1 with
-            | 0 => match (next_level f) with
-                   | f' => S (inv_ack_worker n f' (n - f' n - 1) cd0') end
-            | S cd1' => inv_ack_worker (n - 1) f cd1' cd0' end
-end.
+  match cd0 with
+  | 0 => 0
+  | 1 => 1
+  | S cd0' =>
+    match cd1 with
+    | 0 => match (next_level f) with
+             f' => S (inv_ack_worker n f' (n - f' n - 1) cd0') end 
+    | S cd1' => inv_ack_worker (n - 1) f cd1' cd0'
+    end
+  end.
 
 Definition inv_ack_helper i n :=
-match (inv_ack_hier i), (inv_ack_hier (S i)) with
-       | f0, f1 => inv_ack_worker (f0 n) f1 (f0 n - f1 n) (f0 n - (i + 3))
-end.
+  match (inv_ack_hier i), (inv_ack_hier (S i)) with
+  | f0, f1 => inv_ack_worker (f0 n) f1 (f0 n - f1 n) (f0 n - (i + 3))
+  end.
 
 Definition inv_ack n :=
-match n with
-| 0 => 0
-| 1 => 0
-| _ => inv_ack_worker (S(S n)) minus_2 2 n
-end.
+  match n with
+  | 0 | 1 => 0
+  | _ => inv_ack_worker (S (S n)) minus_2 2 n
+  end.
 
-
-Theorem inv_ack_interstate_1 : forall n f cd1 cd0 k, (k <= cd1) -> (k < cd0)
--> inv_ack_worker n f cd1 cd0 = inv_ack_worker (n - k) f (cd1 - k) (cd0 - k).
+Theorem inv_ack_interstate_1 : forall n f cd1 cd0 k,
+    k <= cd1 ->
+    k < cd0 ->
+    inv_ack_worker n f cd1 cd0 = inv_ack_worker (n - k) f (cd1 - k) (cd0 - k).
 Proof.
-intros n f cd1 cd0 k. generalize dependent cd0.
-generalize dependent cd1. generalize dependent n.
-induction k. { intros. repeat rewrite minus_n_0. trivial. }
-intros n cd1 cd0 HSk1 HSk0.
-destruct cd0. { omega. } destruct cd0. { omega. }
-destruct cd1. { omega. }
-rewrite <- le_S_n_m in HSk1. rewrite <- lt_S_n_m in HSk0.
-apply (IHk (n - 1) cd1 (S cd0)) in HSk1.
-repeat rewrite <- minus_S. rewrite <- sub_add_distr in HSk1.
-unfold plus in HSk1. rewrite <- HSk1. trivial. trivial.
+  intros n f cd1 cd0 k. generalize dependent cd0.
+  generalize dependent cd1. generalize dependent n.
+  induction k.
+  - intros. repeat rewrite minus_n_0. trivial.
+  - intros n cd1 cd0 HSk1 HSk0.
+    destruct cd0; [omega|].
+    destruct cd0; [omega|].
+    destruct cd1; [omega|].
+    rewrite <- le_S_n_m in HSk1. rewrite <- lt_S_n_m in HSk0.
+    apply (IHk (n - 1) cd1 (S cd0)) in HSk1; trivial.
+    repeat rewrite <- minus_S. rewrite <- sub_add_distr in HSk1.
+    unfold plus in HSk1. rewrite <- HSk1; trivial.
 Qed.
-
 
 Theorem inv_ack_interstate_2 : forall n f cd1 cd0,
-(1 <= cd0) -> inv_ack_worker n f cd1 cd0
-= S (inv_ack_worker (n - cd1) (next_level f)
-     ((n - cd1) - (next_level f (n - cd1)) - 1) (cd0 - cd1 - 1)).
+    1 <= cd0 ->
+    inv_ack_worker n f cd1 cd0 =
+    S (inv_ack_worker (n - cd1) (next_level f)
+                      ((n - cd1) - (next_level f (n - cd1)) - 1) (cd0 - cd1 - 1)).
 Proof.
-intros n f cd1 cd0 H. remember (cd0 - cd1) as m.
-destruct m.
-{ rewrite (inv_ack_interstate_1 _ _ _ _ (cd0 - 1)). simpl.
-  rewrite sub_compl. trivial. trivial. omega. omega. }
-rewrite (inv_ack_interstate_1 _ _ _ _ cd1).
-rewrite Nat.sub_diag.
-destruct m. { simpl. rewrite <- Heqm. trivial. }
-rewrite <- Heqm. rewrite <- minus_S. rewrite minus_n_0. trivial.
-trivial. omega.
+  intros n f cd1 cd0 H. remember (cd0 - cd1) as m.
+  destruct m.
+  - rewrite (inv_ack_interstate_1 _ _ _ _ (cd0 - 1)); [|omega..].
+    simpl. rewrite sub_compl; trivial.
+  - rewrite (inv_ack_interstate_1 _ _ _ _ cd1); [|trivial | omega].
+    rewrite Nat.sub_diag.
+    destruct m; [simpl; rewrite <- Heqm; trivial|]. 
+    rewrite <- Heqm. rewrite <- minus_S. rewrite minus_n_0. trivial.
 Qed.
-
 
 Theorem inv_ack_interstate_3 : forall i n, 
-(i + 4 <= inv_ack_hier i n) -> inv_ack_helper i n = 1 + inv_ack_helper (S i) n.
+    i + 4 <= inv_ack_hier i n ->
+    inv_ack_helper i n = 1 + inv_ack_helper (S i) n.
 Proof.
-intros i n Hin.
-unfold inv_ack_helper. remember (inv_ack_hier i) as f0.
-remember (inv_ack_hier (S i)) as f1. remember (inv_ack_hier (S(S i))) as f2.
-assert (4 <= n) as Hn.
-{ assert (H := (inv_ack_hier_each_shrink i n)). rewrite <- Heqf0 in H. omega. }
-assert (f1 n <= f0 n).
-{ rewrite Heqf1. rewrite Heqf0. apply inv_ack_hier_shrink. omega. }
-rewrite inv_ack_interstate_2. simpl.
-replace (f0 n - (f0 n - f1 n)) with (f1 n).
-assert (f2 = next_level f1) as Hf12. { rewrite Heqf1. rewrite Heqf2. trivial. }
-rewrite <- Hf12.
-rewrite <- sub_add_distr. replace (f2 (f1 n) + 1) with (f2 n).
-replace (f0 n - (i + 3) - (f0 n - f1 n) - 1) with (f1 n - S (i + 3)).
-- trivial.
-- rewrite <- sub_sub_comm. rewrite <- (sub_add_distr _ (i + 3) _).
-  rewrite (plus_comm 1 _). rewrite <- sub_sub_comm. omega.
-- rewrite Hf12. rewrite plus_comm.
-  rewrite next_level_interstate_2. trivial.
-  rewrite Heqf1. apply inv_ack_hier_each_shrink. omega.
-- omega.
-- omega.
+  intros i n Hin.
+  unfold inv_ack_helper. remember (inv_ack_hier i) as f0.
+  remember (inv_ack_hier (S i)) as f1. remember (inv_ack_hier (S(S i))) as f2.
+  assert (4 <= n) as Hn by
+        (assert (H := (inv_ack_hier_each_shrink i n)); rewrite <- Heqf0 in H; omega).
+  assert (f1 n <= f0 n) by
+      (rewrite Heqf1; rewrite Heqf0; apply inv_ack_hier_shrink; omega). 
+  rewrite inv_ack_interstate_2; [|omega].
+  replace (f0 n - (f0 n - f1 n)) with (f1 n); [|omega].
+  assert (f2 = next_level f1) as Hf12; [rewrite Heqf1, Heqf2; trivial|]. 
+  rewrite <- Hf12, <- sub_add_distr.
+  replace (f2 (f1 n) + 1) with (f2 n).
+  replace (f0 n - (i + 3) - (f0 n - f1 n) - 1) with (f1 n - S (i + 3)).
+  - trivial.
+  - rewrite <- sub_sub_comm, <- (sub_add_distr _ (i + 3) _), 
+    (plus_comm 1 _), <- sub_sub_comm. omega.
+  - rewrite Hf12. rewrite plus_comm.
+    rewrite next_level_interstate_2; [trivial| |omega].
+    rewrite Heqf1. apply inv_ack_hier_each_shrink.
 Qed.
-
 
 Theorem inv_ack_interstate_4 : forall n,
-(2 <= n) -> inv_ack n = 1 + inv_ack_helper 0 (S(S n)).
+    2 <= n ->
+    inv_ack n = 1 + inv_ack_helper 0 (S (S n)).
 Proof.
-intro. unfold inv_ack_helper. simpl.
-destruct n. { omega. } destruct n. { omega. }
-assert (S(S(S(S n))) - 2 = S(S n)). { omega. }
-intro. clear H0. unfold inv_ack. rewrite inv_ack_interstate_2.
-rewrite H. rewrite <- sub_add_distr. rewrite <- sub_add_distr.
-rewrite plus_comm. rewrite <- minus_2_correct in H.
-rewrite <- H. rewrite <- (next_level_interstate_2 minus_2 _). trivial.
-apply minus_2_shrink. omega. omega.
+  intro. unfold inv_ack_helper. simpl.
+  destruct n; [omega|].
+  destruct n; [omega|].
+  assert (S (S (S (S n))) - 2 = S (S n)) by omega.
+  intro. clear H0. unfold inv_ack.
+  rewrite inv_ack_interstate_2 by omega.
+  rewrite H. rewrite <- sub_add_distr. rewrite <- sub_add_distr.
+  rewrite plus_comm. rewrite <- minus_2_correct in H.
+  rewrite <- H, <- (next_level_interstate_2 minus_2 _);
+    [trivial | apply minus_2_shrink | omega].
 Qed.
 
-
-Theorem inv_ack_helper_thm : forall i k n, (3 <= n) ->
-(i + k + 4 <= inv_ack_hier (i + k) n) <-> (S i <= inv_ack_helper k n).
+Theorem inv_ack_helper_thm : forall i k n,
+    3 <= n ->
+    i + k + 4 <= inv_ack_hier (i + k) n <->
+    S i <= inv_ack_helper k n.
 Proof.
-intros i k n Hn. generalize dependent k.
-
-assert (forall k, k + 4 <= inv_ack_hier k n <-> 1 <= inv_ack_helper k n) as H0.
-{ split. intro. rewrite inv_ack_interstate_3. omega. trivial.
-  unfold inv_ack_helper. intro. simpl. rewrite not_lt. rewrite plus_comm.
-  simpl. rewrite lt_succ_r. intro. assert (inv_ack_hier k n - (k + 3) = 0).
-  { omega. } rewrite H1 in H. simpl in H. inversion H. }
-
-induction i. { apply H0. }
-intro. specialize (IHi (S k)). replace (i + S k) with (S i + k) in IHi.
-split.
-- intro. assert (H1 := H). rewrite IHi in H. rewrite inv_ack_interstate_3. omega.
-  apply (Nat.le_trans _ (inv_ack_hier (S i + k) n) _).
-  apply (Nat.le_trans _ (S i + k + 4) _). omega. trivial.
-  apply inv_ack_hier_shrink_gen. trivial. omega.
-- intro. rewrite IHi. rewrite inv_ack_interstate_3 in H. omega.
-  rewrite H0. omega.
-- omega.
+  intros i k n Hn. generalize dependent k.
+  (** maybe make this a lemma? *)
+  assert (forall k, k + 4 <= inv_ack_hier k n <-> 1 <= inv_ack_helper k n) as H0.
+  { split.
+    - intro. rewrite inv_ack_interstate_3; [omega | trivial].
+    - unfold inv_ack_helper. intro. rewrite not_lt. rewrite plus_comm.
+      simpl. rewrite lt_succ_r. intro.
+      assert (inv_ack_hier k n - (k + 3) = 0) by omega.
+      rewrite H1 in H; simpl in H; inversion H. }
+  induction i; [apply H0|]. 
+  intro. specialize (IHi (S k)).
+  replace (i + S k) with (S i + k) in IHi by omega.
+  split.
+  - intro. assert (H1 := H). rewrite IHi in H.
+    rewrite inv_ack_interstate_3; [omega|].
+    apply (Nat.le_trans _ (inv_ack_hier (S i + k) n) _).
+    + apply (Nat.le_trans _ (S i + k + 4) _); [omega | trivial].
+    + apply inv_ack_hier_shrink_gen; [trivial | omega].
+  - intro. rewrite IHi. rewrite inv_ack_interstate_3 in H;
+                          [|rewrite H0]; omega.
 Qed.
 
+Theorem inv_ack_correct' : forall x n, (inv_ack n <= x <-> n <= Ack x x).
+Proof.
+  destruct n; [simpl; omega|]. 
+  destruct n.
+  - simpl. destruct x; [simpl; omega|].
+    rewrite inv_ack_Ack. simpl. split.
+    + intro. apply (Nat.le_trans _ (inv_ack_hier 0 3) _).
+      * apply inv_ack_hier_shrink_gen; [trivial | omega].
+      * simpl. omega.
+    + intro. omega. 
+  - rewrite inv_ack_interstate_4. destruct x. { simpl. omega. }
+                                              rewrite <- le_S_n_m. rewrite inv_ack_Ack.
+    rewrite not_lt. rewrite not_lt.
+    rewrite <- le_succ_l. rewrite <- le_succ_l.
+    replace x with (x + 0). replace (S (S (x + 0) + 2)) with (x + 0 + 4).
+    rewrite (inv_ack_helper_thm x 0 _). rewrite (plus_comm _ 2). simpl.
+    omega. omega. omega. omega. omega.
+Qed.
 
 Theorem inv_ack_correct : forall x n, (inv_ack n <= x <-> n <= Ack x x).
 Proof.
-destruct n. { simpl. omega. }
-destruct n.
-{
-simpl. destruct x. simpl. omega.
-rewrite inv_ack_Ack. simpl. split.
-- intro. apply (Nat.le_trans _ (inv_ack_hier 0 3) _).
-  apply inv_ack_hier_shrink_gen. trivial. omega. simpl. omega.
-- intro. omega. }
-rewrite inv_ack_interstate_4. destruct x. { simpl. omega. }
-rewrite <- le_S_n_m. rewrite inv_ack_Ack.
-rewrite not_lt. rewrite not_lt.
-rewrite <- le_succ_l. rewrite <- le_succ_l.
-replace x with (x + 0). replace (S (S (x + 0) + 2)) with (x + 0 + 4).
-rewrite (inv_ack_helper_thm x 0 _). rewrite (plus_comm _ 2). simpl.
-omega. omega. omega. omega. omega.
+  destruct n; [simpl; omega|]. 
+  destruct n.
+  - simpl. destruct x; [simpl; omega|].
+    rewrite inv_ack_Ack. simpl. split.
+    + intro. apply (Nat.le_trans _ (inv_ack_hier 0 3) _).
+      * apply inv_ack_hier_shrink_gen; [trivial | omega].
+      * simpl. omega.
+    + intro. omega. 
+  - rewrite inv_ack_interstate_4 by omega.
+    destruct x; [simpl; omega |]. 
+    rewrite <- le_S_n_m. rewrite inv_ack_Ack.
+    repeat rewrite not_lt. rewrite <- le_succ_l, <- le_succ_l.
+    replace x with (x + 0) by omega.
+    replace (S (S (x + 0) + 2)) with (x + 0 + 4) by omega.
+    rewrite (inv_ack_helper_thm x 0 _) by omega.
+    rewrite (plus_comm _ 2). simpl; omega.
 Qed.
 
-
 Fixpoint sum_f (f : nat -> nat) (k n : nat) :=
-match k with
-| 0 => n
-| S k' => n + sum_f f k' (f n)
-end.
+  match k with
+  | 0 => n
+  | S k' => n + sum_f f k' (f n)
+  end.
 
 Definition HS n := match (inv_ack_hier 2), (inv_ack_hier 3 n) with
-| f, m => m + sum_f f (m - 1) (f n) end.
+                   | f, m => m + sum_f f (m - 1) (f n) end.
 
 Compute HS 5.
 Compute HS 6.
